theories/soundness.v
@@ -8,6 +8,10 @@ Module soundness
   (Import conv : conv_sig lattice syntax par ieq)
   (Import typing : typing_sig lattice syntax par ieq conv)
   (Import lr : lr_sig lattice syntax par ieq conv).
+
+Module pfacts := par_facts lattice syntax par.
+Import pfacts.
+
 (* Semantic substitution well-formedness *)
 Definition ρ_ok Γ Δ ρ := forall i ℓ A, lookup i Γ ℓ A -> forall m PA, ⟦ c2e Δ ⊨ A [ρ] ⟧ m ↘ PA -> PA ℓ (ρ i).
 
@@ -106,465 +110,488 @@ Qed.
 
 (* Fundamental theorem: Syntactic typing implies semantic typing *)
 Theorem soundness :
-  (forall Γ a A, Γ ⊢ a ∈ A -> Γ ⊨ a ∈ A) /\
-  (forall Γ, ⊢ Γ -> ⊨ Γ).
+  (forall Γ ℓ a A, Wt Γ ℓ a A -> SemWt Γ ℓ a A) /\
+  (forall Γ, Wff Γ -> SemWff Γ).
 Proof.
   apply wt_mutual.
   (* Var *)
-  - move => Γ i A h ih l ρ hρ.
-    move /(_ i ltac:(done) ltac:(auto)) in ih.
-    case : ih => j ih.
+  - move => Γ ℓ0 ℓ i A h ih l hℓ Ξ ρ hρ.
+    rewrite /SemWff in ih.
+    move /ih : (l) {ih} => [ℓ1 [j ih]].
     rewrite SemWt_Univ in ih.
-    move: (ih _ hρ) => [PA h1].
-    exists j. exists PA. split. auto.
-    move: (hρ _ _ l _ _ h1).
-    by asimpl.
+    move /ih : (hρ) => {ih} [? [PA h1]].
+    exists j, PA. split. auto.
+    move /hρ : h1 l => /[apply].
+    asimpl.
+    (* Need subsumption *)
+    admit.
   (* Pi *)
-  - move => Γ i A B _ /SemWt_Univ h0 _ /SemWt_Univ h1.
+  - move => Γ i ℓ ℓ0 A B _ /SemWt_Univ h0 _ /SemWt_Univ h1.
     apply SemWt_Univ.
-    move => ρ hρ.
-    move /(_ ρ hρ) : h0; intros (PA & hPA).
-    eexists => /=.
-    apply InterpUnivN_Fun_nopf; eauto.
-    move => *; asimpl. eauto using ρ_ok_cons.
+    move => Ξ ρ hρ.
+    move /(_ Ξ ρ hρ) : h0; intros (? & PA & hPA).
+    split.
+    + admit.
+    + eexists => //=.
+      apply InterpUnivN_Fun_nopf; eauto.
+      move => *; asimpl.
+      hauto lq:on use:ρ_ok_cons.
   (* Abs *)
-  - move => Γ A b B i _ /SemWt_Univ hB _ hb ρ hρ.
-    case /(_ ρ hρ) : hB => /= PPi hPPi.
+  - move => Γ ℓ ℓ0 ℓ1 A b B i _ /SemWt_Univ hB _ hb Δ ρ hρ.
+    move /(_ _ ρ hρ) : hB => /= [? [PPi hPPi]].
     exists i, PPi. split => //.
     move /InterpUnivN_Fun_inv_nopf : hPPi.
-    intros (PA & hPA & hTot & ?). subst.
+    move => [PA][?][hTot]?. subst.
     rewrite /ProdSpace.
-    move => a PB ha. asimpl => hPB.
-    have : ρ_ok (A :: Γ) (a .: ρ) by eauto using ρ_ok_cons.
+    split.
+    + admit.
+    + move => a PB ha. asimpl => hPB.
+    have : ρ_ok ((ℓ0, A) :: Γ) Δ (a .: ρ) by eauto using ρ_ok_cons.
     move /hb.
     intros (m & PB0 & hPB0 & hPB0').
     replace PB0 with PB in * by hauto l:on use:InterpUnivN_deterministic'.
-    qauto l:on use:P_AppAbs_cbn,InterpUnivN_back_clos  solve+:(by asimpl).
+    apply : InterpUnivN_back_clos; eauto.
+    admit.
+    apply : P_AppAbs_cbn. by asimpl.
   (* App *)
-  - move => Γ f A B b _ ihf _ ihb ρ hρ.
+  - move => Γ ℓ ℓ0 f A B b _ ihf _ ihb Δ ρ hρ.
     rewrite /SemWt in ihf ihb.
-    move /(_ ρ hρ) : ihf; intros (i & PPi & hPi & hf).
-    move /(_ ρ hρ) : ihb; intros (j & PA & hPA & hb).
+    move /(_ _ _ hρ) : ihf; intros (i & PPi & hPi & hf).
+    move /(_ _ _ hρ) : ihb; intros (j & PA & hPA & hb).
     simpl in hPi.
     move /InterpUnivN_Fun_inv_nopf : hPi. intros (PA0 & hPA0 & hTot & ?). subst.
     have ? : PA0 = PA by eauto using InterpUnivN_deterministic'. subst.
-    move  : hf (hb) => /[apply].
+    move : hf => [?].
+    move  : (hb) => /[swap] /[apply].
     move : hTot hb. move/[apply].
     asimpl. hauto lq:on.
   (* Conv *)
-  - move => Γ a A B i _ hA _ /SemWt_Univ hB ? ρ hρ.
-    have hs : subst_tm ρ A <: subst_tm ρ B
-      by hauto l:on use:Sub_morphing.
+  - move => Γ ℓ ℓ0 a A B i _ hA _ /SemWt_Univ hB ? Δ ρ hρ.
+    have hs : conv (c2e Δ) (subst_tm ρ A) (subst_tm ρ B)
+      by admit.
+      (* by hauto l:on use:Sub_morphing. *)
     move /hB : (hρ) {hB}.
-    move => [PB]hPB.
+    move => [?][PB]hPB.
     move /hA : hρ {hA}.
     move => [j][PA][hPA]ha.
-    have : PB a[ρ] by hauto q:on use:InterpUnivN_Sub.
+    have ? : ⟦ c2e Δ ⊨ A[ρ] ⟧ i ↘ PB by eauto using InterpUnivN_Conv.
+    have : PA = PB by eauto using InterpUnivN_deterministic'.
     hauto lq:on.
-  (* Zero *)
-  - hauto l:on.
-  (* Suc *)
-  - move => Γ a _ ha _ hΓ ρ hρ.
-    move /(_ ρ hρ) : ha.
-    move => [m][PA][h] h0.
-    exists m, PA. split=>//.
-    move /InterpUnivN_Nat_inv in h.
-    hauto lq:on use:S_Suc.
-  (* Ind *)
-  - move => Γ a b c A l _ /SemWt_Univ hA _ ha _ hb _ hc ρ hρ.
-    move /(_ ρ hρ) : ha => [m][PA][ha0]ha1.
-    move /(_ ρ hρ) : hc => [n][PA0][/InterpUnivN_Nat_inv ->][v[hc1 hc2]]/=.
-    asimpl.
-    set bs := (X in tInd _ X _).
-    move : {c} (c[ρ]) hc1 hc2.
-    apply is_nat_val_ind => {v}.
-    + move => ? ? c hc _. subst.
-      exists m, PA. split.
-      * apply : InterpUnivN_back_preservation_star;eauto.
-        asimpl.
-        qauto l:on use:Pars_morphing_star,good_Pars_morphing_ext ctrs:rtc.
-      * simpl.
-        apply : InterpUnivN_back_clos_star; eauto.
-        by apply P_IndZero_star.
-    + move => ? a0 ? ih c hc ha. subst.
-      move /(_ a0 ltac:(apply rtc_refl) ha) : ih => [m0][PA1][hPA1]hr.
-      have hρ' : ρ_ok (tNat :: Γ) (a0 .: ρ).
-      {
-        apply : ρ_ok_cons; auto.
-        apply InterpUnivN_Nat.
-        hauto lq:on ctrs:rtc.
-      }
-      have : ρ_ok (A :: tNat :: Γ) ((tInd a[ρ] bs a0) .: (a0 .: ρ))
-        by eauto using ρ_ok_cons.
-      move /hb => {hb} [m1][PA2][hPA2]h.
-      exists m1, PA2.
-      split.
-      * move : hPA2. asimpl.
-        move /InterpUnivN_back_preservation_star. apply.
-        qauto l:on use:Pars_morphing_star,good_Pars_morphing_ext ctrs:rtc.
-      * move : h.
-        move /InterpUnivN_back_clos_star. apply; eauto.
-        subst bs.
-        apply : P_IndSuc_star'; eauto.
-        by asimpl.
-    + move => a0 ? <- _ a1 *.
-      have ? : wne a1 by hauto lq:on.
-      suff  /hA : ρ_ok (tNat :: Γ) (a1 .: ρ).
-      move => [S hS].
-      exists l, S. split=>//.
-      suff ? : wn bs.
-      have ? : wn a[ρ] by sfirstorder use:adequacy.
-      have : wne (tInd a[ρ] bs a1) by auto using wne_ind.
-      eapply adequacy; eauto.
+  (* (* Zero *) *)
+  (* - hauto l:on. *)
+  (* (* Suc *) *)
+  (* - move => Γ a _ ha _ hΓ ρ hρ. *)
+  (*   move /(_ ρ hρ) : ha. *)
+  (*   move => [m][PA][h] h0. *)
+  (*   exists m, PA. split=>//. *)
+  (*   move /InterpUnivN_Nat_inv in h. *)
+  (*   hauto lq:on use:S_Suc. *)
+  (* (* Ind *) *)
+  (* - move => Γ a b c A l _ /SemWt_Univ hA _ ha _ hb _ hc ρ hρ. *)
+  (*   move /(_ ρ hρ) : ha => [m][PA][ha0]ha1. *)
+  (*   move /(_ ρ hρ) : hc => [n][PA0][/InterpUnivN_Nat_inv ->][v[hc1 hc2]]/=. *)
+  (*   asimpl. *)
+  (*   set bs := (X in tInd _ X _). *)
+  (*   move : {c} (c[ρ]) hc1 hc2. *)
+  (*   apply is_nat_val_ind => {v}. *)
+  (*   + move => ? ? c hc _. subst. *)
+  (*     exists m, PA. split. *)
+  (*     * apply : InterpUnivN_back_preservation_star;eauto. *)
+  (*       asimpl. *)
+  (*       qauto l:on use:Pars_morphing_star,good_Pars_morphing_ext ctrs:rtc. *)
+  (*     * simpl. *)
+  (*       apply : InterpUnivN_back_clos_star; eauto. *)
+  (*       by apply P_IndZero_star. *)
+  (*   + move => ? a0 ? ih c hc ha. subst. *)
+  (*     move /(_ a0 ltac:(apply rtc_refl) ha) : ih => [m0][PA1][hPA1]hr. *)
+  (*     have hρ' : ρ_ok (tNat :: Γ) (a0 .: ρ). *)
+  (*     { *)
+  (*       apply : ρ_ok_cons; auto. *)
+  (*       apply InterpUnivN_Nat. *)
+  (*       hauto lq:on ctrs:rtc. *)
+  (*     } *)
+  (*     have : ρ_ok (A :: tNat :: Γ) ((tInd a[ρ] bs a0) .: (a0 .: ρ)) *)
+  (*       by eauto using ρ_ok_cons. *)
+  (*     move /hb => {hb} [m1][PA2][hPA2]h. *)
+  (*     exists m1, PA2. *)
+  (*     split. *)
+  (*     * move : hPA2. asimpl. *)
+  (*       move /InterpUnivN_back_preservation_star. apply. *)
+  (*       qauto l:on use:Pars_morphing_star,good_Pars_morphing_ext ctrs:rtc. *)
+  (*     * move : h. *)
+  (*       move /InterpUnivN_back_clos_star. apply; eauto. *)
+  (*       subst bs. *)
+  (*       apply : P_IndSuc_star'; eauto. *)
+  (*       by asimpl. *)
+  (*   + move => a0 ? <- _ a1 *. *)
+  (*     have ? : wne a1 by hauto lq:on. *)
+  (*     suff  /hA : ρ_ok (tNat :: Γ) (a1 .: ρ). *)
+  (*     move => [S hS]. *)
+  (*     exists l, S. split=>//. *)
+  (*     suff ? : wn bs. *)
+  (*     have ? : wn a[ρ] by sfirstorder use:adequacy. *)
+  (*     have : wne (tInd a[ρ] bs a1) by auto using wne_ind. *)
+  (*     eapply adequacy; eauto. *)
 
-      subst bs.
-      rewrite /SemWt in hb.
-      have /hA : ρ_ok (tNat :: Γ) (var_tm 0 .: ρ).
-      {
-        apply : ρ_ok_cons; auto.
-        apply InterpUnivN_Nat.
-        hauto lq:on ctrs:rtc.
-      }
-      move => [S1 hS1].
-      have /hb : ρ_ok (A :: tNat :: Γ) (var_tm 0 .: (var_tm 0 .: ρ)).
-      {
-        apply : ρ_ok_cons; cycle 2; eauto.
-        apply : ρ_ok_cons; cycle 2; eauto.
-        apply InterpUnivN_Nat.
-        hauto lq:on ctrs:rtc.
-        hauto q:on ctrs:rtc use:adequacy.
-      }
-      move =>[m0][PA1][h1]h2.
-      have : wn b[var_tm 0 .: (var_tm 0 .: ρ)] by hauto q:on use:adequacy.
-      clear => h.
-      apply wn_antirenaming with (ξ :=  var_zero .: (var_zero .: id)).
-      by asimpl.
+  (*     subst bs. *)
+  (*     rewrite /SemWt in hb. *)
+  (*     have /hA : ρ_ok (tNat :: Γ) (var_tm 0 .: ρ). *)
+  (*     { *)
+  (*       apply : ρ_ok_cons; auto. *)
+  (*       apply InterpUnivN_Nat. *)
+  (*       hauto lq:on ctrs:rtc. *)
+  (*     } *)
+  (*     move => [S1 hS1]. *)
+  (*     have /hb : ρ_ok (A :: tNat :: Γ) (var_tm 0 .: (var_tm 0 .: ρ)). *)
+  (*     { *)
+  (*       apply : ρ_ok_cons; cycle 2; eauto. *)
+  (*       apply : ρ_ok_cons; cycle 2; eauto. *)
+  (*       apply InterpUnivN_Nat. *)
+  (*       hauto lq:on ctrs:rtc. *)
+  (*       hauto q:on ctrs:rtc use:adequacy. *)
+  (*     } *)
+  (*     move =>[m0][PA1][h1]h2. *)
+  (*     have : wn b[var_tm 0 .: (var_tm 0 .: ρ)] by hauto q:on use:adequacy. *)
+  (*     clear => h. *)
+  (*     apply wn_antirenaming with (ξ :=  var_zero .: (var_zero .: id)). *)
+  (*     by asimpl. *)
 
-      apply : ρ_ok_cons; auto.
-      apply InterpUnivN_Nat.
-      hauto lq:on use:adequacy db:nfne.
-  (* Bool *)
-  - hauto l:on use:SemWt_Univ.
+  (*     apply : ρ_ok_cons; auto. *)
+  (*     apply InterpUnivN_Nat. *)
+  (*     hauto lq:on use:adequacy db:nfne. *)
+  (* (* Bool *) *)
+  (* - hauto l:on use:SemWt_Univ. *)
   (* Univ *)
-  - hauto lq:on use:InterpUnivN_Univ, SemWt_Univ.
-  (* Refl *)
-  - move => Γ a A _ _ _ ha ρ.
-    move : ha. move/[apply]. move => [m [PA [h0 h1]]].
-    exists 0. eexists.
-    split => /=.
-    + apply InterpUnivN_Eq;
-      hauto l:on use:adequacy, InterpUniv_wn_ty, InterpUnivN_Eq unfold:CR.
-    + qauto l:on ctrs:rtc use:Coherent_reflexive inv:Par .
-  (* Eq *)
-  - move => Γ a b A i j _ ha _ hb _ /SemWt_Univ hA.
-    apply SemWt_Univ => ρ hρ.
-    eexists => /=. apply InterpUnivN_Eq;
-      hauto l:on use:adequacy, InterpUniv_wn_ty unfold:SemWt, CR.
-  (* J *)
-  - move => Γ t a b p A i j C _ ha _ hb _ _ _ hp _ /SemWt_Univ hC _ ht ρ hρ.
-    move : hp (hρ); move/[apply] => /=. intros (m & PA & hPA & hp).
-    move  /InterpUnivN_Eq_inv : hPA. intros (-> & ? & ? & ?).
-    move : ht (hρ); move/[apply]. intros (k & PA & hPA & ht).
-    move : hp.
-    move =>[[hp hco] | ?].
-    + exists k, PA.
-      split.
-      * asimpl in hPA.
-        apply : InterpUnivN_Coherent; eauto.
-        rewrite /Coherent.
-        case : hco => ab ?.
-        exists (subst_tm (tRefl .: (ab .: ρ)) C).
-        split.
-        ** apply Pars_morphing_star; last by apply rtc_refl.
-           apply good_Pars_morphing_ext2;
-             hauto lq:on ctrs:rtc.
-        ** apply Pars_morphing_star; last by apply rtc_refl.
-           apply good_Pars_morphing_ext2. apply rtc_refl.
-           tauto. apply rtc_refl.
-      * asimpl.
-        eapply InterpUnivN_back_clos_star with (b := subst_tm ρ t); eauto.
-        sfirstorder use: P_JRefl_star.
-    + asimpl.
-      move /(_ (subst_tm ρ p .: (subst_tm ρ b .: ρ))) : hC.
-      case.
-      * eapply ρ_ok_cons with (i := 0).
-        asimpl.
-        apply InterpUnivN_Eq; eauto.
-        right. auto.
-        move : hb (hρ). move/[apply].
-        move => [i0 [PA0 hb0]].
-        hauto l:on use:ρ_ok_cons.
-      * move => PC hPC.
-        exists i, PC. split; first tauto.
-        qauto l:on use:adequacy,wne_j unfold:CR.
-  (* Sig *)
-  - move => Γ i A B _ /SemWt_Univ h0 _ /SemWt_Univ h1.
-    apply SemWt_Univ.
-    move => ρ hρ.
-    move /(_ ρ hρ) : h0; intros (PA & hPA).
-    eexists => /=.
-    apply InterpUnivN_Sig_nopf; eauto.
-    move => *; asimpl. eauto using ρ_ok_cons.
-  (* Pack *)
-  - move => Γ a A b B i _ ha _ hb _ /SemWt_Univ hB ρ hρ.
-    move /ha : (hρ) => [m][PA][ha0]ha1.
-    move /hb : (hρ) => [m0][PB][hb0]hb1.
-    move /hB : (hρ) => [S]/=hS.
-    exists i, S => /=.
-    split => //.
-    move /InterpUnivN_Sig_inv_nopf : hS => [PA0][hPA0][hPB0]?. subst.
-    rewrite /SumSpace.
-    left. do 2 eexists. split; first by apply rtc_refl.
-    have ? : PA = PA0 by eauto using InterpUnivN_deterministic'. subst.
-    split => // PB0. asimpl.
-    move /hPB0 :ha1.
-    move => [PB1]. asimpl => *.
-    asimpl in hb0.
-    have [*] : PB = PB1 /\ PB0 = PB1 by  eauto using InterpUnivN_deterministic'.
-    congruence.
-  (* Let Pack *)
-  - move => Γ t b A B C i _ _ _ _ _ _ ht _ hb _ /SemWt_Univ hC ρ hρ.
-    move /ht : (hρ) {ht} => [m][PA][/= /[dup] hSig /InterpUnivN_Sig_inv_nopf].
-    move => [PA0][h0][h1]?. subst.
-    rewrite /SumSpace.
-    case.
-    + move => [a0][b0][h2][h3]h4.
-      have : ρ_ok (tSig A B :: Γ) ((tPack a0 b0) .: ρ) by
-        hauto  use:ρ_ok_cons,InterpUnivN_Sig_nopf  unfold:SumSpace.
-      move /hC => [S] hS {hC}.
-      exists i, S. split=>//.
-      asimpl.
-      move /InterpUnivN_back_preservation_star : (hS). apply.
-      qauto l:on use:Pars_morphing_star,good_Pars_morphing_ext ctrs:rtc.
-      apply : InterpUnivN_back_clos_star; eauto.
-      apply P_LetPack_star; eauto.
-      asimpl.
-      have ?: ρ_ok (A :: Γ) (a0 .: ρ) by eauto using ρ_ok_cons.
-      move /h1 : (h3) => [PB] /[dup] hPB.
-      move /h4 => ?.
-      asimpl in hPB.
-      have : ρ_ok (B :: A :: Γ) (b0 .: (a0 .: ρ)) by eauto using ρ_ok_cons.
-      move /hb => [m0][PA]. asimpl. move => [hPA] hPA0.
-      by have <- : PA = S by eauto using InterpUnivN_deterministic'.
-    + move => h.
-      have /hC : ρ_ok (tSig A B :: Γ) (t[ρ] .: ρ) by
-        apply : ρ_ok_cons; hauto lq:on use:adequacy.
-      move => [S hS].
-      exists i, S. asimpl; split => //.
-      set a := (X in S X).
-      suff : wne a by hauto q:on use:adequacy.
-      subst a.
-      apply wne_let=>//.
-      have hz : wne (var_tm 0) by hauto lq:on ctrs:rtc.
-      have hz' : PA0 (var_tm 0) by move : h0 hz; clear; hauto lq:on use:adequacy unfold:CR.
-      apply wn_antirenaming with (ξ := var_zero .: (var_zero .: id)).
-      asimpl.
-      have hρ' : ρ_ok (A :: Γ) (var_tm 0 .: ρ) by eauto using ρ_ok_cons.
-      move /h1 : hz' => [PB /ltac:(asimpl) hPB].
-      have hz'' : PB (var_tm 0) by move : hPB hz; clear; hauto lq:on use:adequacy unfold:CR.
-      have : ρ_ok (B :: A :: Γ) (var_tm 0 .: (var_tm 0 .: ρ)) by eauto using ρ_ok_cons.
-      move /hb. clear.
-      hauto l:on use:adequacy unfold:CR.
+  - move => Γ ℓ i _ hΓ.
+    rewrite SemWt_Univ.
+    move => Ξ ρ hρ.
+    split.
+    admit.
+    eexists=>/=.
+    apply : InterpUnivN_Univ. lia.
+  (* (* Refl *) *)
+  (* - move => Γ a A _ _ _ ha ρ. *)
+  (*   move : ha. move/[apply]. move => [m [PA [h0 h1]]]. *)
+  (*   exists 0. eexists. *)
+  (*   split => /=. *)
+  (*   + apply InterpUnivN_Eq; *)
+  (*     hauto l:on use:adequacy, InterpUniv_wn_ty, InterpUnivN_Eq unfold:CR. *)
+  (*   + qauto l:on ctrs:rtc use:Coherent_reflexive inv:Par . *)
+  (* (* Eq *) *)
+  (* - move => Γ a b A i j _ ha _ hb _ /SemWt_Univ hA. *)
+  (*   apply SemWt_Univ => ρ hρ. *)
+  (*   eexists => /=. apply InterpUnivN_Eq; *)
+  (*     hauto l:on use:adequacy, InterpUniv_wn_ty unfold:SemWt, CR. *)
+  (* (* J *) *)
+  (* - move => Γ t a b p A i j C _ ha _ hb _ _ _ hp _ /SemWt_Univ hC _ ht ρ hρ. *)
+  (*   move : hp (hρ); move/[apply] => /=. intros (m & PA & hPA & hp). *)
+  (*   move  /InterpUnivN_Eq_inv : hPA. intros (-> & ? & ? & ?). *)
+  (*   move : ht (hρ); move/[apply]. intros (k & PA & hPA & ht). *)
+  (*   move : hp. *)
+  (*   move =>[[hp hco] | ?]. *)
+  (*   + exists k, PA. *)
+  (*     split. *)
+  (*     * asimpl in hPA. *)
+  (*       apply : InterpUnivN_Coherent; eauto. *)
+  (*       rewrite /Coherent. *)
+  (*       case : hco => ab ?. *)
+  (*       exists (subst_tm (tRefl .: (ab .: ρ)) C). *)
+  (*       split. *)
+  (*       ** apply Pars_morphing_star; last by apply rtc_refl. *)
+  (*          apply good_Pars_morphing_ext2; *)
+  (*            hauto lq:on ctrs:rtc. *)
+  (*       ** apply Pars_morphing_star; last by apply rtc_refl. *)
+  (*          apply good_Pars_morphing_ext2. apply rtc_refl. *)
+  (*          tauto. apply rtc_refl. *)
+  (*     * asimpl. *)
+  (*       eapply InterpUnivN_back_clos_star with (b := subst_tm ρ t); eauto. *)
+  (*       sfirstorder use: P_JRefl_star. *)
+  (*   + asimpl. *)
+  (*     move /(_ (subst_tm ρ p .: (subst_tm ρ b .: ρ))) : hC. *)
+  (*     case. *)
+  (*     * eapply ρ_ok_cons with (i := 0). *)
+  (*       asimpl. *)
+  (*       apply InterpUnivN_Eq; eauto. *)
+  (*       right. auto. *)
+  (*       move : hb (hρ). move/[apply]. *)
+  (*       move => [i0 [PA0 hb0]]. *)
+  (*       hauto l:on use:ρ_ok_cons. *)
+  (*     * move => PC hPC. *)
+  (*       exists i, PC. split; first tauto. *)
+  (*       qauto l:on use:adequacy,wne_j unfold:CR. *)
+  (* (* Sig *) *)
+  (* - move => Γ i A B _ /SemWt_Univ h0 _ /SemWt_Univ h1. *)
+  (*   apply SemWt_Univ. *)
+  (*   move => ρ hρ. *)
+  (*   move /(_ ρ hρ) : h0; intros (PA & hPA). *)
+  (*   eexists => /=. *)
+  (*   apply InterpUnivN_Sig_nopf; eauto. *)
+  (*   move => *; asimpl. eauto using ρ_ok_cons. *)
+  (* (* Pack *) *)
+  (* - move => Γ a A b B i _ ha _ hb _ /SemWt_Univ hB ρ hρ. *)
+  (*   move /ha : (hρ) => [m][PA][ha0]ha1. *)
+  (*   move /hb : (hρ) => [m0][PB][hb0]hb1. *)
+  (*   move /hB : (hρ) => [S]/=hS. *)
+  (*   exists i, S => /=. *)
+  (*   split => //. *)
+  (*   move /InterpUnivN_Sig_inv_nopf : hS => [PA0][hPA0][hPB0]?. subst. *)
+  (*   rewrite /SumSpace. *)
+  (*   left. do 2 eexists. split; first by apply rtc_refl. *)
+  (*   have ? : PA = PA0 by eauto using InterpUnivN_deterministic'. subst. *)
+  (*   split => // PB0. asimpl. *)
+  (*   move /hPB0 :ha1. *)
+  (*   move => [PB1]. asimpl => *. *)
+  (*   asimpl in hb0. *)
+  (*   have [*] : PB = PB1 /\ PB0 = PB1 by  eauto using InterpUnivN_deterministic'. *)
+  (*   congruence. *)
+  (* (* Let Pack *) *)
+  (* - move => Γ t b A B C i _ _ _ _ _ _ ht _ hb _ /SemWt_Univ hC ρ hρ. *)
+  (*   move /ht : (hρ) {ht} => [m][PA][/= /[dup] hSig /InterpUnivN_Sig_inv_nopf]. *)
+  (*   move => [PA0][h0][h1]?. subst. *)
+  (*   rewrite /SumSpace. *)
+  (*   case. *)
+  (*   + move => [a0][b0][h2][h3]h4. *)
+  (*     have : ρ_ok (tSig A B :: Γ) ((tPack a0 b0) .: ρ) by *)
+  (*       hauto  use:ρ_ok_cons,InterpUnivN_Sig_nopf  unfold:SumSpace. *)
+  (*     move /hC => [S] hS {hC}. *)
+  (*     exists i, S. split=>//. *)
+  (*     asimpl. *)
+  (*     move /InterpUnivN_back_preservation_star : (hS). apply. *)
+  (*     qauto l:on use:Pars_morphing_star,good_Pars_morphing_ext ctrs:rtc. *)
+  (*     apply : InterpUnivN_back_clos_star; eauto. *)
+  (*     apply P_LetPack_star; eauto. *)
+  (*     asimpl. *)
+  (*     have ?: ρ_ok (A :: Γ) (a0 .: ρ) by eauto using ρ_ok_cons. *)
+  (*     move /h1 : (h3) => [PB] /[dup] hPB. *)
+  (*     move /h4 => ?. *)
+  (*     asimpl in hPB. *)
+  (*     have : ρ_ok (B :: A :: Γ) (b0 .: (a0 .: ρ)) by eauto using ρ_ok_cons. *)
+  (*     move /hb => [m0][PA]. asimpl. move => [hPA] hPA0. *)
+  (*     by have <- : PA = S by eauto using InterpUnivN_deterministic'. *)
+  (*   + move => h. *)
+  (*     have /hC : ρ_ok (tSig A B :: Γ) (t[ρ] .: ρ) by *)
+  (*       apply : ρ_ok_cons; hauto lq:on use:adequacy. *)
+  (*     move => [S hS]. *)
+  (*     exists i, S. asimpl; split => //. *)
+  (*     set a := (X in S X). *)
+  (*     suff : wne a by hauto q:on use:adequacy. *)
+  (*     subst a. *)
+  (*     apply wne_let=>//. *)
+  (*     have hz : wne (var_tm 0) by hauto lq:on ctrs:rtc. *)
+  (*     have hz' : PA0 (var_tm 0) by move : h0 hz; clear; hauto lq:on use:adequacy unfold:CR. *)
+  (*     apply wn_antirenaming with (ξ := var_zero .: (var_zero .: id)). *)
+  (*     asimpl. *)
+  (*     have hρ' : ρ_ok (A :: Γ) (var_tm 0 .: ρ) by eauto using ρ_ok_cons. *)
+  (*     move /h1 : hz' => [PB /ltac:(asimpl) hPB]. *)
+  (*     have hz'' : PB (var_tm 0) by move : hPB hz; clear; hauto lq:on use:adequacy unfold:CR. *)
+  (*     have : ρ_ok (B :: A :: Γ) (var_tm 0 .: (var_tm 0 .: ρ)) by eauto using ρ_ok_cons. *)
+  (*     move /hb. clear. *)
+  (*     hauto l:on use:adequacy unfold:CR. *)
+
+  (* Void *)
+  - hauto lq:on ctrs:IOk use:InterpUnivN_Void, SemWt_Univ.
+  (* Absurd *)
+  - hauto lq:on use:InterpUnivN_Void_inv unfold:SemWt.
   (* Nil *)
   - apply SemWff_nil.
   (* Cons *)
   - eauto using SemWff_cons.
-Qed.
+Admitted.
 
-Lemma mltt_normalizing Γ a A : Γ ⊢ a ∈ A -> wn a /\ wn A.
-Proof.
-  move /(proj1 soundness) /(_ var_tm).
-  elim.
-  - asimpl.
-    hauto l:on use:adequacy, InterpUniv_wn_ty unfold:CR.
-  - rewrite /ρ_ok=>i ? m PA. asimpl.
-    hauto q:on ctrs:rtc use:adequacy.
-Qed.
+(* Lemma mltt_normalizing Γ a A : Γ ⊢ a ∈ A -> wn a /\ wn A. *)
+(* Proof. *)
+(*   move /(proj1 soundness) /(_ var_tm). *)
+(*   elim. *)
+(*   - asimpl. *)
+(*     hauto l:on use:adequacy, InterpUniv_wn_ty unfold:CR. *)
+(*   - rewrite /ρ_ok=>i ? m PA. asimpl. *)
+(*     hauto q:on ctrs:rtc use:adequacy. *)
+(* Qed. *)
 
-(* Need to prove something about scoping before we can recover consistency *)
-Inductive stm (n : nat) : tm -> Prop :=
-| SC_Var i :
-  i < n ->
-  (* ----- *)
-  stm n (var_tm i)
+(* (* Need to prove something about scoping before we can recover consistency *) *)
+(* Inductive stm (n : nat) : tm -> Prop := *)
+(* | SC_Var i : *)
+(*   i < n -> *)
+(*   (* ----- *) *)
+(*   stm n (var_tm i) *)
 
-| SC_Abs b :
-  stm (S n) b ->
-  (* ------------ *)
-  stm n (tAbs b)
+(* | SC_Abs b : *)
+(*   stm (S n) b -> *)
+(*   (* ------------ *) *)
+(*   stm n (tAbs b) *)
 
-| SC_App a b :
-  stm n a ->
-  stm n b ->
-  (* ---------- *)
-  stm n (tApp a b)
+(* | SC_App a b : *)
+(*   stm n a -> *)
+(*   stm n b -> *)
+(*   (* ---------- *) *)
+(*   stm n (tApp a b) *)
 
-| SC_Pi A B :
-  stm n A ->
-  stm (S n) B ->
-  (* ------------ *)
-  stm n (tPi A B)
+(* | SC_Pi A B : *)
+(*   stm n A -> *)
+(*   stm (S n) B -> *)
+(*   (* ------------ *) *)
+(*   stm n (tPi A B) *)
 
-| SC_Univ i :
-  (* ----------- *)
-  stm n (tUniv i)
+(* | SC_Univ i : *)
+(*   (* ----------- *) *)
+(*   stm n (tUniv i) *)
 
-| SC_Zero :
-  (* --------- *)
-  stm n tZero
+(* | SC_Zero : *)
+(*   (* --------- *) *)
+(*   stm n tZero *)
 
-| SC_Suc a :
-  stm n a ->
-  (* -------------- *)
-  stm n (tSuc a)
+(* | SC_Suc a : *)
+(*   stm n a -> *)
+(*   (* -------------- *) *)
+(*   stm n (tSuc a) *)
 
-| SC_Nat :
-  (* -------------- *)
-  stm n tNat
+(* | SC_Nat : *)
+(*   (* -------------- *) *)
+(*   stm n tNat *)
 
-| SC_Eq a b A :
-  stm n a ->
-  stm n b ->
-  stm n A ->
-  (* ---------------- *)
-  stm n (tEq a b A)
+(* | SC_Eq a b A : *)
+(*   stm n a -> *)
+(*   stm n b -> *)
+(*   stm n A -> *)
+(*   (* ---------------- *) *)
+(*   stm n (tEq a b A) *)
 
-| SC_J t a b p :
-  stm n t ->
-  stm n a ->
-  stm n b ->
-  stm n p ->
-  (* ------------- *)
-  stm n (tJ t a b p)
+(* | SC_J t a b p : *)
+(*   stm n t -> *)
+(*   stm n a -> *)
+(*   stm n b -> *)
+(*   stm n p -> *)
+(*   (* ------------- *) *)
+(*   stm n (tJ t a b p) *)
 
-| SC_Ind a b c :
-  stm n a ->
-  stm (2 + n) b ->
-  stm n c ->
-  stm n (tInd a b c)
+(* | SC_Ind a b c : *)
+(*   stm n a -> *)
+(*   stm (2 + n) b -> *)
+(*   stm n c -> *)
+(*   stm n (tInd a b c) *)
 
-| SC_Refl :
-  (* --------- *)
-  stm n tRefl
+(* | SC_Refl : *)
+(*   (* --------- *) *)
+(*   stm n tRefl *)
 
-| SC_Pack a b :
-  stm n a ->
-  stm n b ->
-  (* ------------- *)
-  stm n (tPack a b)
+(* | SC_Pack a b : *)
+(*   stm n a -> *)
+(*   stm n b -> *)
+(*   (* ------------- *) *)
+(*   stm n (tPack a b) *)
 
-| SC_Sig A B :
-  stm n A ->
-  stm (S n) B ->
-  (* ------------ *)
-  stm n (tSig A B)
+(* | SC_Sig A B : *)
+(*   stm n A -> *)
+(*   stm (S n) B -> *)
+(*   (* ------------ *) *)
+(*   stm n (tSig A B) *)
 
-| SC_Let a b :
-  stm n a ->
-  stm (S (S n)) b ->
-  (* -------------- *)
-  stm n (tLet a b).
+(* | SC_Let a b : *)
+(*   stm n a -> *)
+(*   stm (S (S n)) b -> *)
+(*   (* -------------- *) *)
+(*   stm n (tLet a b). *)
 
-#[export]Hint Constructors stm : stm.
+(* #[export]Hint Constructors stm : stm. *)
 
 
-Lemma scope_lt n a : stm n a -> forall m, n <= m -> stm m a.
-Proof. move => h. elim : a / h; hauto lq:on ctrs:stm solve+:lia. Qed.
+(* Lemma scope_lt n a : stm n a -> forall m, n <= m -> stm m a. *)
+(* Proof. move => h. elim : a / h; hauto lq:on ctrs:stm solve+:lia. Qed. *)
 
-Lemma ne_scope a : ne a -> forall n, stm n a -> n > 0.
-Proof. elim : a; hauto q:on inv:stm b:on solve+:lia. Qed.
+(* Lemma ne_scope a : ne a -> forall n, stm n a -> n > 0. *)
+(* Proof. elim : a; hauto q:on inv:stm b:on solve+:lia. Qed. *)
 
-Lemma lookup_lt i A Γ : lookup i Γ A -> i < length Γ.
-Proof. move => h. elim : i Γ A / h; sfirstorder. Qed.
+(* Lemma lookup_lt i A Γ : lookup i Γ A -> i < length Γ. *)
+(* Proof. move => h. elim : i Γ A / h; sfirstorder. Qed. *)
 
-Lemma wt_scope Γ a A : Γ ⊢ a ∈ A -> stm (length Γ) a.
-Proof. move => h. elim : Γ a A / h; hauto use:lookup_lt q:on ctrs:stm. Qed.
+(* Lemma wt_scope Γ a A : Γ ⊢ a ∈ A -> stm (length Γ) a. *)
+(* Proof. move => h. elim : Γ a A / h; hauto use:lookup_lt q:on ctrs:stm. Qed. *)
 
-Lemma scope_ren_up n m ξ :
-  (forall i, i < n -> ξ i < m) ->  forall i, i < S n -> upRen_tm_tm ξ i < S m.
-Proof.
-  move => h.
-  case => [|p].
-  - asimpl. lia.
-  - move : (h p). asimpl. lia.
-Qed.
+(* Lemma scope_ren_up n m ξ : *)
+(*   (forall i, i < n -> ξ i < m) ->  forall i, i < S n -> upRen_tm_tm ξ i < S m. *)
+(* Proof. *)
+(*   move => h. *)
+(*   case => [|p]. *)
+(*   - asimpl. lia. *)
+(*   - move : (h p). asimpl. lia. *)
+(* Qed. *)
 
-Lemma scope_renaming n a (h : stm n a) :
-  forall m ξ, (forall i, i < n -> ξ i < m) -> stm m (ren_tm ξ a).
-Proof.
-  elim : a / h=>//=; eauto 10 using scope_ren_up with stm.
-Qed.
+(* Lemma scope_renaming n a (h : stm n a) : *)
+(*   forall m ξ, (forall i, i < n -> ξ i < m) -> stm m (ren_tm ξ a). *)
+(* Proof. *)
+(*   elim : a / h=>//=; eauto 10 using scope_ren_up with stm. *)
+(* Qed. *)
 
-Lemma scope_weaken m a : stm m a -> stm (S m) (ren_tm shift a).
-Proof. move /scope_renaming. apply. lia. Qed.
+(* Lemma scope_weaken m a : stm m a -> stm (S m) (ren_tm shift a). *)
+(* Proof. move /scope_renaming. apply. lia. Qed. *)
 
-Lemma scope_morphing_up n m ρ :
-  (forall i, i < n -> stm m (ρ i)) ->
-  forall i, i < S n -> stm (S m) (up_tm_tm ρ i).
-Proof.
-  move => h.
-  case.
-  asimpl. hauto lq:on ctrs:stm solve+:lia.
-  hauto lq:on use:scope_weaken simp+:asimpl solve+:lia.
-Qed.
+(* Lemma scope_morphing_up n m ρ : *)
+(*   (forall i, i < n -> stm m (ρ i)) -> *)
+(*   forall i, i < S n -> stm (S m) (up_tm_tm ρ i). *)
+(* Proof. *)
+(*   move => h. *)
+(*   case. *)
+(*   asimpl. hauto lq:on ctrs:stm solve+:lia. *)
+(*   hauto lq:on use:scope_weaken simp+:asimpl solve+:lia. *)
+(* Qed. *)
 
-Lemma scope_morphing n a (h : stm n a) :
-  forall m ρ, (forall i, i < n -> stm m (ρ i)) -> stm m (subst_tm ρ a).
-Proof.
-  elim : n a / h=>//=; eauto 10 using scope_morphing_up with stm.
-Qed.
+(* Lemma scope_morphing n a (h : stm n a) : *)
+(*   forall m ρ, (forall i, i < n -> stm m (ρ i)) -> stm m (subst_tm ρ a). *)
+(* Proof. *)
+(*   elim : n a / h=>//=; eauto 10 using scope_morphing_up with stm. *)
+(* Qed. *)
 
-Lemma scope_subst n a b (h : stm (S n) a) (h0 : stm n b) :
-  stm n (subst_tm (b..) a).
-Proof.
-  apply scope_morphing with (n := S n)=>//.
-  case.
-  by asimpl. move => p. asimpl.
-  hauto lq:on ctrs:stm solve+:lia.
-Qed.
+(* Lemma scope_subst n a b (h : stm (S n) a) (h0 : stm n b) : *)
+(*   stm n (subst_tm (b..) a). *)
+(* Proof. *)
+(*   apply scope_morphing with (n := S n)=>//. *)
+(*   case. *)
+(*   by asimpl. move => p. asimpl. *)
+(*   hauto lq:on ctrs:stm solve+:lia. *)
+(* Qed. *)
 
-Lemma Par_scope a b (h : a ⇒ b) : forall n, stm n a -> stm n b.
-Proof.
-  elim : a b / h;
-    match goal with
-    | [|-context[subst_tm]] => idtac
-    | _ => hauto lq:on inv:stm ctrs:stm
-    end.
-  - hauto lq:on inv:stm ctrs:stm use:scope_subst.
-  - move => a0 a1 b0 b1 c0 c1 ha iha hb ihb hc ihc n hi.
-    inversion hi; subst.
-    apply scope_morphing with (n := 2 +  n);simpl;  eauto.
-    case => [_|].
-    + hauto lq:on inv:stm ctrs:stm.
-    + case => [_|]/=.
-      hauto lq:on inv:stm.
-      move => n0 h.
-      have {h}: n0 < n by lia.
-      hauto lq:on ctrs:stm.
-  - move => a0 a1 b0 b1 c0 c1 ha iha hb ihb hc ihc n hi.
-    inversion hi; subst.
-    apply scope_morphing with (n := 2 +  n);simpl;  eauto.
-    case => [_|].
-    + asimpl. apply ihb. move : hi. clear. qauto l:on inv:stm.
-    + case => [_|]/=. apply iha.
-      move : hi. clear. qauto l:on inv:stm.
-      move => m h.
-      have {}h : m < n by lia.
-      hauto lq:on ctrs:stm.
-Qed.
+(* Lemma Par_scope a b (h : a ⇒ b) : forall n, stm n a -> stm n b. *)
+(* Proof. *)
+(*   elim : a b / h; *)
+(*     match goal with *)
+(*     | [|-context[subst_tm]] => idtac *)
+(*     | _ => hauto lq:on inv:stm ctrs:stm *)
+(*     end. *)
+(*   - hauto lq:on inv:stm ctrs:stm use:scope_subst. *)
+(*   - move => a0 a1 b0 b1 c0 c1 ha iha hb ihb hc ihc n hi. *)
+(*     inversion hi; subst. *)
+(*     apply scope_morphing with (n := 2 +  n);simpl;  eauto. *)
+(*     case => [_|]. *)
+(*     + hauto lq:on inv:stm ctrs:stm. *)
+(*     + case => [_|]/=. *)
+(*       hauto lq:on inv:stm. *)
+(*       move => n0 h. *)
+(*       have {h}: n0 < n by lia. *)
+(*       hauto lq:on ctrs:stm. *)
+(*   - move => a0 a1 b0 b1 c0 c1 ha iha hb ihb hc ihc n hi. *)
+(*     inversion hi; subst. *)
+(*     apply scope_morphing with (n := 2 +  n);simpl;  eauto. *)
+(*     case => [_|]. *)
+(*     + asimpl. apply ihb. move : hi. clear. qauto l:on inv:stm. *)
+(*     + case => [_|]/=. apply iha. *)
+(*       move : hi. clear. qauto l:on inv:stm. *)
+(*       move => m h. *)
+(*       have {}h : m < n by lia. *)
+(*       hauto lq:on ctrs:stm. *)
+(* Qed. *)
 
-Lemma Pars_scope a b (h : a ⇒* b) : forall n, stm n a -> stm n b.
-Proof. elim : a b / h; sfirstorder use:Par_scope. Qed.
+(* Lemma Pars_scope a b (h : a ⇒* b) : forall n, stm n a -> stm n b. *)
+(* Proof. elim : a b / h; sfirstorder use:Par_scope. Qed. *)
 
-Lemma consistency a : ~ nil ⊢ a ∈ tEq tZero (tSuc tZero) tNat.
-Proof.
-  move => /[dup] /wt_scope /= h.
-  move /(proj1 soundness).
-  rewrite /SemWt.
-  have : ρ_ok nil var_tm by
-    hauto lq:on inv:lookup unfold:ρ_ok.
-  move/[swap]/[apply].
-  move => [m][PA][].
-  move /InterpUnivN_Eq_inv => [->]_[[_/Coherent_consistent]|[v[/Pars_scope]]]//.
-  asimpl. move /(_ 0 h). move/ne_scope/[apply]. lia.
-Qed.
+(* Lemma consistency a : ~ nil ⊢ a ∈ tEq tZero (tSuc tZero) tNat. *)
+(* Proof. *)
+(*   move => /[dup] /wt_scope /= h. *)
+(*   move /(proj1 soundness). *)
+(*   rewrite /SemWt. *)
+(*   have : ρ_ok nil var_tm by *)
+(*     hauto lq:on inv:lookup unfold:ρ_ok. *)
+(*   move/[swap]/[apply]. *)
+(*   move => [m][PA][]. *)
+(*   move /InterpUnivN_Eq_inv => [->]_[[_/Coherent_consistent]|[v[/Pars_scope]]]//. *)
+(*   asimpl. move /(_ 0 h). move/ne_scope/[apply]. lia. *)
+(* Qed. *)
